src/tls/TLSConstants.fst
@@ -10,26 +10,28 @@ module TLSConstants
 
 #set-options "--max_fuel 0 --initial_fuel 0 --max_ifuel 1 --initial_ifuel 1"
 
-//NS, JP: TODO, this include should eventually move to TLSMem, when that module exists
-include FStar.HyperStack.All
-
-let type_of (#a : Type) (x : a) : Type = a
-
-(* Start Hacks *)
-// assume val empty_bytes : FStar.Bytes.lbytes 0
-(* End Hacks *)
 open FStar.String
 open FStar.Seq
 open FStar.Date
 open FStar.Bytes
 open FStar.Error
 open TLSError
-//open CoreCrypto // avoid?!
-
 
 module HS = FStar.HyperStack
 
-include Parse // carving out basic formatting code to break a dependency.
+//NS, JP: TODO, this include should eventually move to TLSMem, when that module exists
+//CF it exists: Mem.fst on verify, but not with this include.
+include FStar.HyperStack.All
+include Parse 
+// carving out basic formatting code to break a dependency.
+
+
+
+
+
+(* FRESH LIBRARY-LIKE FUNCTIONS; RELOCATE? *)
+
+let type_of (#a : Type) (x : a) : Type = a
 
 let rec fold_string (#a:Type)
                     (f: a -> string)
@@ -94,21 +96,35 @@ let rec forall_aux (#a:Type) (#b:Type) (env:b) (f: b -> a -> Tot bool) (l:list a
     | hd::tl -> if f env hd then forall_aux env f tl else false
 
 let mem_rev (#a:eqtype) (l:list a) (x:a) = List.Tot.mem x l
-(** Polarity for reading and writing *)
-type rw =
-  | Reader
-  | Writer
 
-(** Role of the library in current execution *)
+
+
+
+
+
+/// HIGH-LEVEL DECLARATIONS
+
+(** Role of the connection endpoints *)
 type role =
   | Client
   | Server
-
-(** Dual role *)
 let dualRole = function
   | Client -> Server
   | Server -> Client
 
+(** Polarity for reading and writing on a connection *)
+type rw =
+  | Reader
+  | Writer
+
+
+
+
+
+
+
+/// 18-02-22 QD fodder?
+/// 
 (** Protocol version negotiated values *)
 type protocolVersion' =
   | SSL_3p0 // supported, with no security guarantees
@@ -120,9 +136,92 @@ type protocolVersion' =
 
 type protocolVersion = pv:protocolVersion'{~(UnknownVersion? pv)}
 
+// aka TLS_1p3
 let is_pv_13 = function
   | TLS_1p3 -> true
   | _ -> false
+
+#set-options "--max_fuel 0 --initial_fuel 0 --max_ifuel 1 --initial_ifuel 1"
+
+(** Serializing function for the protocol version *)
+val versionBytes: protocolVersion' -> Tot (lbytes 2)
+let versionBytes pv =
+  match pv with
+  | SSL_3p0 -> twobytes ( 3z, 0z)
+  | TLS_1p0 -> twobytes ( 3z, 1z)
+  | TLS_1p1 -> twobytes ( 3z, 2z )
+  | TLS_1p2 -> twobytes ( 3z, 3z )
+  | TLS_1p3 -> twobytes ( 3z, 4z )
+  | UnknownVersion a b -> twobytes ( a, b )
+
+(** Parsing function for the protocol version *)
+val parseVersion: pinverse_t versionBytes
+let parseVersion v =
+  match cbyte2 v with
+  | ( 3z, 0z ) -> Correct SSL_3p0
+  | ( 3z, 1z ) -> Correct TLS_1p0
+  | ( 3z, 2z ) -> Correct TLS_1p1
+  | ( 3z, 3z ) -> Correct TLS_1p2
+  | ( 3z, 4z ) -> Correct TLS_1p3
+  | ( a,  b  ) -> Correct (UnknownVersion a b)
+
+val inverse_version: x:_ -> Lemma
+  (requires True)
+  (ensures lemma_inverse_g_f versionBytes parseVersion x)
+  [SMTPat (parseVersion (versionBytes x))]
+let inverse_version x = ()
+
+val pinverse_version: x:_ -> Lemma
+  (requires True)
+  (ensures (lemma_pinverse_f_g Bytes.equal versionBytes parseVersion x))
+  [SMTPat (versionBytes (Correct?._0 (parseVersion x)))]
+let pinverse_version x = ()
+
+// DRAFT#23
+// to be used *only* in ServerHello.version.
+// https://tlswg.github.io/tls13-spec/#rfc.section.4.2.1
+let draft = 23z
+let versionBytes_draft: protocolVersion -> Tot (lbytes 2) = function
+  | TLS_1p3 -> twobytes ( 127z, draft )
+  | pv -> versionBytes pv
+val parseVersion_draft: pinverse_t versionBytes_draft
+let parseVersion_draft v =
+  match cbyte2 v with
+  | (127z, d) ->
+      if d = draft
+      then Correct TLS_1p3
+      else Error(AD_decode_error, "Refused to parse unknown draft "^print_bytes v^": expected TLS 1.3#"^UInt8.to_string draft)
+  | (3z, 4z) -> Error(AD_decode_error, "Refused to parse TLS 1.3 final version: expected TLS 1.3#"^UInt8.to_string draft)
+  | _ ->
+    match parseVersion v with
+    | Correct (UnknownVersion _ _) -> Error(AD_decode_error, "Parsed unknown version ")
+    | Correct pv -> Correct pv
+    | Error z -> Error z
+
+(** Determine the oldest protocol versions for TLS *)
+let minPV (a:protocolVersion) (b:protocolVersion) =
+  match a,b with
+  | SSL_3p0, _  | _, SSL_3p0 -> SSL_3p0
+  | TLS_1p0, _  | _, TLS_1p0 -> TLS_1p0
+  | TLS_1p1, _  | _, TLS_1p1 -> TLS_1p1
+  | TLS_1p2, _  | _, TLS_1p2 -> TLS_1p2
+  | TLS_1p3, _  | _, TLS_1p3 -> TLS_1p3
+
+let geqPV a b = (b = minPV a b)
+
+let string_of_pv = function
+  | SSL_3p0 -> "SSL3"
+  | TLS_1p0 -> "1.0"
+  | TLS_1p1 -> "1.1"
+  | TLS_1p2 -> "1.2"
+  | TLS_1p3 -> "1.3"
+  | UnknownVersion a b -> "Unknown protocol version: " ^ (print_bytes (twobytes (a, b)))
+
+
+
+
+
+/// Various elements used in ciphersuites 
 
 (* Key exchange algorithms *)
 type kexAlg =
@@ -149,7 +248,6 @@ type encAlg =
   | Block of blockCipher
   | Stream of streamCipher
 
-
 type hash_alg = Hashing.Spec.alg
 
 (** TLS-specific hash algorithms *)
@@ -165,12 +263,11 @@ type macAlg =
   | HMac     of hash_alg
   | SSLKHash of hash_alg_classic
 
-
 (** Authenticated Encryption modes *)
 type aeAlg =
   | MACOnly: hash_alg -> aeAlg
   | MtE: encAlg -> hash_alg -> aeAlg
-  | AEAD: aeadAlg -> hash_alg -> aeAlg  // the hash algorithm is for the ciphersuite; it is not used by the record layer.
+  | AEAD: aeadAlg -> hash_alg -> aeAlg // the hash algorithm is for the ciphersuite; it is not used by the record layer.
 
 let aeAlg_hash = function
   | MACOnly ha -> ha
@@ -185,7 +282,6 @@ let lhae = function
 (** Sequence numbers for StreamAE/StatefulLHAE *)
 let is_seqn (n:nat) = repr_bytes n <= 8
 type seqn_t = n:nat { is_seqn n }
-
 
 (** Predicates for Strong Authentication *)
 // MtE: ``The AE algorithms are CPA and INT-CTXT''
@@ -203,21 +299,68 @@ let strongAEAlg _ _ = false
 
 assume val strongAuthAE: pv:protocolVersion -> ae:aeAlg -> Lemma(strongAEAlg pv ae ==> strongAuthAlg pv ae)
 
+//CF we leave these functions abstract for verification purposes
+//CF we may need to be more negative on weak algorithms (so that we don't try to verify their use)
+//CF and more precise/positive on algorithms we implement (so that we reflect lower assumptions)
+
+(** Encryption key sizes *)
+let encKeySize =
+  let open CoreCrypto in function
+  | Stream RC4_128      -> 16
+  | Block TDES_EDE_CBC  -> 24
+  | Block AES_128_CBC   -> 16
+  | Block AES_256_CBC   -> 32
+  | Block TDES_EDE_CBC  -> 24
+  | Block AES_128_CBC   -> 16
+  | Block AES_256_CBC   -> 32
+
+(** AEAD salt sizes *)
+let aeadSaltSize =
+  let open CoreCrypto in function // TLS 1.3 IV salt.
+  | AES_128_GCM       -> 4
+  | AES_256_GCM       -> 4
+  | CHACHA20_POLY1305 -> 12
+  | _                 -> 4 //recheck
+
+(** AEAD *)
+let aeadRecordIVSize =
+  let open CoreCrypto in function // TLS 1.2 explicit IVs
+  | AES_128_GCM       -> 8
+  | AES_256_GCM       -> 8
+  | CHACHA20_POLY1305 -> 0
+  | _                 -> 8 //recheck
+
+(** Hash sizes *)
+val hashSize: h:hashAlg{h<>NULL} -> Tot nat
+let hashSize = function
+  | Hash a  -> Hashing.Spec.tagLen a
+  | MD5SHA1 -> 16 + 20
+
+(** MAC key sizes *)
+let macKeySize = function
+  | HMac alg
+  | SSLKHash alg -> hashSize (Hash alg)
+
+(** MAC sizes *)
+let macSize = function
+  | HMac alg
+  | SSLKHash alg -> hashSize (Hash alg)
+
+
 // -----------------------------------------------------------------------
 // record-layer length constants [5.2.1]
 // note that TLS 1.3 lowers a bit the upper bound of cipher lengths (Ok in principle)
 // but still enables padding beyond plausible plaintext lengths.
 
 (** Constants for API and protocol-level fragments are in [0..2^14] *)
-let max_TLSPlaintext_fragment_length = 16384
-let max_TLSCompressed_fragment_length = max_TLSPlaintext_fragment_length + 1024
-let max_TLSCiphertext_fragment_length = max_TLSPlaintext_fragment_length + 2048
+let max_TLSPlaintext_fragment_length     = 16384
+let max_TLSCompressed_fragment_length    = max_TLSPlaintext_fragment_length + 1024
+let max_TLSCiphertext_fragment_length    = max_TLSPlaintext_fragment_length + 2048
 let max_TLSCiphertext_fragment_length_13 = max_TLSPlaintext_fragment_length + 256
 
-//CF we leave these functions abstract for verification purposes
-//CF we may need to be more negative on weak algorithms (so that we don't try to verify their use)
-//CF and more precise/positive on algorithms we implement (so that we reflect lower assumptions)
 
+/// 18-02-22 QD fodder
+/// 
 (** Signature algorithms *)
 type sigAlg = CoreCrypto.sig_alg
 
@@ -306,7 +449,7 @@ let signatureSchemeBytes_is_injective
 : Lemma
   (requires (signatureSchemeBytes s1 == signatureSchemeBytes s2))
   (ensures (s1 == s2))
-= if (SIG_UNKNOWN? s1) = (SIG_UNKNOWN? s2)
+= if SIG_UNKNOWN? s1 = SIG_UNKNOWN? s2
   then ()
   else assume (s1 == s2) // TODO: strengthen int_of_bytes vs. twobytes
 
@@ -395,80 +538,14 @@ let signatureScheme_of_sigHashAlg sa ha =
     int_of_bytes_of_int #2 0x0000;
     SIG_UNKNOWN (bytes_of_int 2 0)
 
-(** Encryption key sizes *)
-let encKeySize =
-  let open CoreCrypto in function
-  | Stream RC4_128      -> 16
-  | Block TDES_EDE_CBC  -> 24
-  | Block AES_128_CBC   -> 16
-  | Block AES_256_CBC   -> 32
-  | Block TDES_EDE_CBC  -> 24
-  | Block AES_128_CBC   -> 16
-  | Block AES_256_CBC   -> 32
 
-(** AEAD salt sizes *)
-let aeadSaltSize =
-  let open CoreCrypto in function // TLS 1.3 IV salt.
-  | AES_128_GCM       -> 4
-  | AES_256_GCM       -> 4
-  | CHACHA20_POLY1305 -> 12
-  | _                 -> 4 //recheck
 
-(** AEAD *)
-let aeadRecordIVSize =
-  let open CoreCrypto in function // TLS 1.2 explicit IVs
-  | AES_128_GCM       -> 8
-  | AES_256_GCM       -> 8
-  | CHACHA20_POLY1305 -> 0
-  | _                 -> 8 //recheck
 
-(** Hash sizes *)
-val hashSize: h:hashAlg{h<>NULL} -> Tot nat
-let hashSize = function
-  | Hash a  -> Hashing.Spec.tagLen a
-  | MD5SHA1 -> 16 + 20
 
-(** MAC key sizes *)
-let macKeySize = function
-  | HMac alg
-  | SSLKHash alg -> hashSize (Hash alg)
 
-(** MAC sizes *)
-let macSize = function
-  | HMac alg
-  | SSLKHash alg -> hashSize (Hash alg)
 
-(** Ciphersuite for SCSV *)
-type scsv_suite =
-  | TLS_EMPTY_RENEGOTIATION_INFO_SCSV
-
-(* let known_cs_list = [( 0x00z, 0x00z ); *)
-(* ( 0x00z, 0x01z );( 0x00z, 0x02z ); ( 0x00z, 0x3Bz ); ( 0x00z, 0x04z ); ( 0x00z, 0x05z ); *)
-(* ( 0x00z, 0x0Az ); ( 0x00z, 0x2Fz ); ( 0x00z, 0x35z ); ( 0x00z, 0x3Cz );( 0x00z, 0x3Dz ); *)
-(*  ( 0x00z, 0x0Dz ); ( 0x00z, 0x10z ); ( 0x00z, 0x13z ); ( 0x00z, 0x16z ); *)
-(*  ( 0x00z, 0x30z ); ( 0x00z, 0x31z ); ( 0x00z, 0x32z ); ( 0x00z, 0x33z ); *)
-(*  ( 0x00z, 0x36z ); ( 0x00z, 0x37z ); ( 0x00z, 0x38z ); ( 0x00z, 0x39z ); *)
-(*  ( 0x00z, 0x3Ez ); ( 0x00z, 0x3Fz ); ( 0x00z, 0x40z ); ( 0x00z, 0x67z ); *)
-(*  ( 0x00z, 0x68z ); ( 0x00z, 0x69z ); ( 0x00z, 0x6Az ); ( 0x00z, 0x6Bz ); *)
-(*  ( 0xc0z, 0x11z ); ( 0xc0z, 0x12z ); ( 0xc0z, 0x13z ); ( 0xc0z, 0x14z ); ( 0xc0z, 0x27z ); ( 0xc0z, 0x28z ); *)
-(*  ( 0xc0z, 0x2fz ); ( 0xc0z, 0x30z ); *)
-(*  ( 0x00z, 0x18z ); ( 0x00z, 0x1Bz ); ( 0x00z, 0x34z ); ( 0x00z, 0x3Az ); ( 0x00z, 0x6Cz ); ( 0x00z, 0x6Dz ); *)
-(* ( 0x00z, 0x9Cz );( 0x00z, 0x9Dz ); *)
-(* ( 0x00z, 0x9Ez );( 0x00z, 0x9Fz );( 0x00z, 0xA0z );( 0x00z, 0xA1z ); *)
-(* ( 0x00z, 0xA2z );( 0x00z, 0xA3z );( 0x00z, 0xA4z );( 0x00z, 0xA5z ); *)
-(* ( 0x00z, 0xA6z ); ( 0x00z, 0xA7z ); ( 0x00z, 0xFFz )] *)
-
-(** Ciphersuite definition *)
-type cipherSuite =
-  | NullCipherSuite: cipherSuite
-  | CipherSuite    : kexAlg -> option sigAlg -> aeAlg -> cipherSuite
-  | CipherSuite13  : aeadAlg -> hash_alg -> cipherSuite
-  | SCSV           : scsv_suite -> cipherSuite
-  | UnknownCipherSuite: a:byte -> b:byte(* {not(List.Tot.contains (a,b) known_cs_list)}  *) -> cipherSuite // JK: incomplete spec
-
-(** List of ciphersuite *)
-type cipherSuites = list cipherSuite
-
+/// QD fodder
+/// 
 (** Compression definition *)
 type compression =
   | NullCompression
@@ -505,7 +582,6 @@ let rec parseCompressions b =
     cm::(parseCompressions b)
   else []
 
-
 #set-options "--max_fuel 1 --initial_fuel 1 --max_ifuel 1 --initial_ifuel 1"
 
 (** Serializing function for lists of compression algorithms *)
@@ -517,84 +593,93 @@ let rec compressionMethodsBytes cms =
   | []   -> empty_bytes
 
 
-#set-options "--max_fuel 0 --initial_fuel 0 --max_ifuel 1 --initial_ifuel 1"
 
-(** Serializing function for the protocol version *)
-val versionBytes: protocolVersion' -> Tot (lbytes 2)
-let versionBytes pv =
-  match pv with
-  | SSL_3p0 -> twobytes ( 3z, 0z)
-  | TLS_1p0 -> twobytes ( 3z, 1z)
-  | TLS_1p1 -> twobytes ( 3z, 2z )
-  | TLS_1p2 -> twobytes ( 3z, 3z )
-  | TLS_1p3 -> twobytes ( 3z, 4z )
-  | UnknownVersion a b -> twobytes ( a, b )
 
-(** Parsing function for the protocol version *)
-val parseVersion: pinverse_t versionBytes
-let parseVersion v =
-  match cbyte2 v with
-  | ( 3z, 0z ) -> Correct SSL_3p0
-  | ( 3z, 1z ) -> Correct TLS_1p0
-  | ( 3z, 2z ) -> Correct TLS_1p1
-  | ( 3z, 3z ) -> Correct TLS_1p2
-  | ( 3z, 4z ) -> Correct TLS_1p3
-  | ( a,  b  ) -> Correct (UnknownVersion a b)
 
-val inverse_version: x:_ -> Lemma
-  (requires True)
-  (ensures lemma_inverse_g_f versionBytes parseVersion x)
-  [SMTPat (parseVersion (versionBytes x))]
-let inverse_version x = ()
 
-val pinverse_version: x:_ -> Lemma
-  (requires True)
-  (ensures (lemma_pinverse_f_g Bytes.equal versionBytes parseVersion x))
-  [SMTPat (versionBytes (Correct?._0 (parseVersion x)))]
-let pinverse_version x = ()
+/// 18-02-22 QD fodder, will require a manual translation as we
+/// primarily use this structured ADT --- see also cipherSuiteName
+/// below, closer to the RFC.
+///
+(** Ciphersuite definition *)
+type cipherSuite =
+  | NullCipherSuite: cipherSuite
+  | CipherSuite    : kexAlg -> option sigAlg -> aeAlg -> cipherSuite
+  | CipherSuite13  : aeadAlg -> hash_alg -> cipherSuite
+  | SCSV           : cipherSuite
+  | UnknownCipherSuite: a:byte -> b:byte(* {not(List.Tot.contains (a,b) known_cs_list)}  *) -> cipherSuite // JK: incomplete spec
 
-// DRAFT#23
-// to be used *only* in ServerHello.version.
-// https://tlswg.github.io/tls13-spec/#rfc.section.4.2.1
-let draft = 23z
-let versionBytes_draft: protocolVersion -> Tot (lbytes 2) = function
-  | TLS_1p3 -> twobytes ( 127z, draft )
-  | pv -> versionBytes pv
-val parseVersion_draft: pinverse_t versionBytes_draft
-let parseVersion_draft v =
-  match cbyte2 v with
-  | (127z, d) ->
-      if d = draft
-      then Correct TLS_1p3
-      else Error(AD_decode_error, "Refused to parse unknown draft "^print_bytes v^": expected TLS 1.3#"^UInt8.to_string draft)
-  | (3z, 4z) -> Error(AD_decode_error, "Refused to parse TLS 1.3 final version: expected TLS 1.3#"^UInt8.to_string draft)
-  | _ ->
-    match parseVersion v with
-    | Correct (UnknownVersion _ _) -> Error(AD_decode_error, "Parsed unknown version ")
-    | Correct pv -> Correct pv
-    | Error z -> Error z
+(** List of ciphersuite *)
+type cipherSuites = list cipherSuite
 
-(** Determine the oldest protocol versions for TLS *)
-let minPV (a:protocolVersion) (b:protocolVersion) =
-  match a,b with
-  | SSL_3p0, _  | _, SSL_3p0 -> SSL_3p0
-  | TLS_1p0, _  | _, TLS_1p0 -> TLS_1p0
-  | TLS_1p1, _  | _, TLS_1p1 -> TLS_1p1
-  | TLS_1p2, _  | _, TLS_1p2 -> TLS_1p2
-  | TLS_1p3, _  | _, TLS_1p3 -> TLS_1p3
+(** Determine if a ciphersuite implies no peer authentication *)
+let isAnonCipherSuite cs =
+  match cs with
+  | CipherSuite Kex_DHE None _ -> true
+  | _ -> false
 
-let geqPV a b = (b = minPV a b)
+(** Determine if a ciphersuite implies using (EC)Diffie-Hellman KEX *)
+let isDHECipherSuite cs =
+  let open CoreCrypto in
+  match cs with
+  | CipherSuite Kex_DHE (Some DSA) _      -> true
+  | CipherSuite Kex_DHE (Some RSASIG) _   -> true
+  | CipherSuite Kex_ECDHE (Some ECDSA) _  -> true
+  | CipherSuite Kex_ECDHE (Some RSASIG) _ -> true
+  | _ -> false
 
-let string_of_pv = function
-  | SSL_3p0 -> "SSL3"
-  | TLS_1p0 -> "1.0"
-  | TLS_1p1 -> "1.1"
-  | TLS_1p2 -> "1.2"
-  | TLS_1p3 -> "1.3"
-  | UnknownVersion a b -> "Unknown protocol version: " ^ (print_bytes (twobytes (a, b)))
+(** Determine if a ciphersuite implies using Elliptic Curves Diffie-Hellman KEX *)
+let isECDHECipherSuite cs =
+  let open CoreCrypto in
+  match cs with
+  | CipherSuite Kex_ECDHE (Some ECDSA) _  -> true
+  | CipherSuite Kex_ECDHE (Some RSASIG) _ -> true
+  | _ -> false
 
-(* JK: injectivity proof requires extra specification for the UnknownCipherSuite objects as they
-   have to be distinct from the 'correct' ones *)
+(** Determine if a ciphersuite implies using plain Diffie-Hellman KEX *)
+let isDHCipherSuite cs =
+  let open CoreCrypto in
+  match cs with
+  | CipherSuite Kex_DH (Some DSA) _    -> true
+  | CipherSuite Kex_DH (Some RSASIG) _ -> true
+  | _ -> false
+
+(** Determine if a ciphersuite implies using an RSA key exchange *)
+let isRSACipherSuite cs =
+  match cs with
+  | CipherSuite Kex_RSA None _ -> true
+  | _ -> false
+
+(** Determine if a ciphersuite implies using MAC only and no encryption *)
+let isOnlyMACCipherSuite cs =
+  match cs with
+  | CipherSuite _ _ (MACOnly _) -> true
+  | _ -> false
+
+(** Determine the signature algorithm associated to a ciphersuite *)
+let sigAlg_of_ciphersuite cs =
+  let open CoreCrypto in
+  match cs with
+  | CipherSuite Kex_RSA None _
+  | CipherSuite Kex_ECDHE (Some RSASIG) _
+  | CipherSuite Kex_DHE (Some RSASIG) _
+  | CipherSuite Kex_DH (Some RSASIG) _   -> RSASIG
+  | CipherSuite Kex_DHE (Some DSA) _
+  | CipherSuite Kex_DH (Some DSA) _      -> DSA
+  | CipherSuite Kex_ECDHE (Some ECDSA) _ -> ECDSA
+  | _ -> unexpected "[sigAlg_of_ciphersuite] invoked on a wrong ciphersuite"
+
+(** Determine if a ciphersuite list contains the SCSV ciphersuite *)
+let contains_SCSV (css: list cipherSuite) = List.Tot.mem SCSV css
+
+/// 18-02-22 The parsers and formatters below are used only in
+/// HandshakeMessages, should move there and disappear
+/// (except for parseCipherSuite, also used in Ticket)
+
+(* JK: injectivity proof requires extra specification for the
+   UnknownCipherSuite objects as they have to be distinct from the
+   'correct' ones *)
+   
 val cipherSuiteBytesOpt: cipherSuite -> Tot (option (lbytes 2))
 let cipherSuiteBytesOpt cs =
   let open CoreCrypto in
@@ -700,7 +785,7 @@ let cipherSuiteBytesOpt cs =
     | CipherSuite Kex_PSK_ECDHE None (AEAD CHACHA20_POLY1305 SHA256)      -> twobytes( 0xccz, 0xacz )
     | CipherSuite Kex_PSK_DHE None (AEAD CHACHA20_POLY1305 SHA256)        -> twobytes( 0xccz, 0xadz )
 
-    | SCSV (TLS_EMPTY_RENEGOTIATION_INFO_SCSV)         -> twobytes ( 0x00z, 0xFFz )
+    | SCSV -> twobytes ( 0x00z, 0xFFz )
     | _ -> None
 
 let validCipherSuite (c:cipherSuite) = Some? (cipherSuiteBytesOpt c)
@@ -713,9 +798,11 @@ let valid_cipher_suites = list valid_cipher_suite
 val cipherSuiteBytes: valid_cipher_suite -> Tot (lbytes 2)
 let cipherSuiteBytes c = Some?.v (cipherSuiteBytesOpt c)
 
+
 #reset-options "--z3rlimit 60 --max_fuel 1 --initial_fuel 1 --max_ifuel 2 --initial_ifuel 2"
 
 (** Auxillary parsing function for ciphersuites *)
+private 
 val parseCipherSuiteAux : lbytes 2 -> Tot (result (c:cipherSuite{validCipherSuite c}))
 let parseCipherSuiteAux b =
   let open CoreCrypto in
@@ -823,7 +910,7 @@ let parseCipherSuiteAux b =
   | ( 0xccz, 0xadz ) -> Correct(CipherSuite Kex_PSK_DHE None (AEAD CHACHA20_POLY1305 SHA256))
 
   (**************************************************************************)
-  | ( 0x00z, 0xFFz ) -> Correct(SCSV (TLS_EMPTY_RENEGOTIATION_INFO_SCSV))
+  | ( 0x00z, 0xFFz ) -> Correct SCSV
   | (b1, b2) -> Correct(UnknownCipherSuite b1 b2)
 // Was:  | _ -> Error(AD_decode_error, perror __SOURCE_FILE__ __LINE__ "Parsed unknown cipher")
 
@@ -842,7 +929,7 @@ val inverse_cipherSuite: x:cipherSuite -> Lemma
   // parse (bytes (Unknown 0 0)) = NullCiphersuite
   // must exclude this case...
   (ensures (let y = cipherSuiteBytesOpt x in
-  (Some? y ==> parseCipherSuiteAux (Some?.v y) = Correct x)))
+    (Some? y ==> parseCipherSuiteAux (Some?.v y) = Correct x)))
   [SMTPat (parseCipherSuiteAux (Some?.v (cipherSuiteBytesOpt x)))]
 let inverse_cipherSuite x = ()
 
@@ -856,7 +943,6 @@ val pinverse_cipherSuite : x:lbytes 2 -> Lemma
                /\ Bytes.equal x (Some?.v (cipherSuiteBytesOpt (Correct?._0 y)))))))
   [SMTPat (cipherSuiteBytesOpt (Correct?._0 (parseCipherSuiteAux x)))]
 let pinverse_cipherSuite x = ()
-
 
 #reset-options
 #set-options "--max_ifuel 1 --initial_ifuel 1 --max_fuel 1 --initial_fuel 1"
@@ -879,13 +965,12 @@ let rec parseCipherSuites b =
     match parseCipherSuites b1 with
       | Correct(css) ->
   (match parseCipherSuite b0 with
-   | Error z ->	Correct css
+   | Error z ->    Correct css
    | Correct cs -> Correct (cs::css))
       | Error z -> Error z
   else
   if length b = 0 then Correct []
   else Error(AD_decode_error, perror __SOURCE_FILE__ __LINE__ "Odd cs bytes number")
-
 
 #reset-options
 #set-options "--max_ifuel 2 --initial_ifuel 2 --max_fuel 2 --initial_fuel 2"
@@ -914,174 +999,14 @@ let rec inverse_cipherSuites x =
 // TODO: We added such constructor, so this is the case now. Prove it.
 
 
-(** Determine if a ciphersuite implies no peer authentication *)
-let isAnonCipherSuite cs =
-  match cs with
-  | CipherSuite Kex_DHE None _ -> true
-  | _ -> false
-
-(** Determine if a ciphersuite implies using (EC)Diffie-Hellman KEX *)
-let isDHECipherSuite cs =
-  let open CoreCrypto in
-  match cs with
-  | CipherSuite Kex_DHE (Some DSA) _      -> true
-  | CipherSuite Kex_DHE (Some RSASIG) _   -> true
-  | CipherSuite Kex_ECDHE (Some ECDSA) _  -> true
-  | CipherSuite Kex_ECDHE (Some RSASIG) _ -> true
-  | _ -> false
-
-(** Determine if a ciphersuite implies using Elliptic Curves Diffie-Hellman KEX *)
-let isECDHECipherSuite cs =
-  let open CoreCrypto in
-  match cs with
-  | CipherSuite Kex_ECDHE (Some ECDSA) _  -> true
-  | CipherSuite Kex_ECDHE (Some RSASIG) _ -> true
-  | _ -> false
-
-(** Determine if a ciphersuite implies using plain Diffie-Hellman KEX *)
-let isDHCipherSuite cs =
-  let open CoreCrypto in
-  match cs with
-  | CipherSuite Kex_DH (Some DSA) _    -> true
-  | CipherSuite Kex_DH (Some RSASIG) _ -> true
-  | _ -> false
-
-(** Determine if a ciphersuite implies using an RSA key exchange *)
-let isRSACipherSuite cs =
-  match cs with
-  | CipherSuite Kex_RSA None _ -> true
-  | _ -> false
-
-(** Determine if a ciphersuite implies using MAC only and no encryption *)
-let isOnlyMACCipherSuite cs =
-  match cs with
-  | CipherSuite _ _ (MACOnly _) -> true
-  | _ -> false
-
-(** Determine the signature algorithm associated to a ciphersuite *)
-let sigAlg_of_ciphersuite cs =
-  let open CoreCrypto in
-  match cs with
-  | CipherSuite Kex_RSA None _
-  | CipherSuite Kex_ECDHE (Some RSASIG) _
-  | CipherSuite Kex_DHE (Some RSASIG) _
-  | CipherSuite Kex_DH (Some RSASIG) _   -> RSASIG
-  | CipherSuite Kex_DHE (Some DSA) _
-  | CipherSuite Kex_DH (Some DSA) _      -> DSA
-  | CipherSuite Kex_ECDHE (Some ECDSA) _ -> ECDSA
-  | _ -> unexpected "[sigAlg_of_ciphersuite] invoked on a wrong ciphersuite"
 
 
-(** Definition for the PRF label type *)
-type prflabel = bytes
-
-(** Key schedule labels *)
-let extract_label          = utf8_encode "master secret"
-let extended_extract_label = utf8_encode "extended master secret"
-let kdf_label              = utf8_encode "key expansion"
-
-(** PRF definitions based on the protocol version *)
-type prePrfAlg =
-  | PRF_SSL3_nested         // MD5(SHA1(...)) for extraction and keygen
-  | PRF_SSL3_concat         // MD5 @| SHA1    for VerifyData tags
-  | PRF_TLS_1p01 of prflabel                       // MD5 xor SHA1
-  | PRF_TLS_1p2 : prflabel -> macAlg -> prePrfAlg  // typically SHA256 but may depend on CS
-  | PRF_TLS_1p3 // TBC
-
-(** PRF associations *)
-//BB.TODO: Documentation ?
-type kefAlg_t = prePrfAlg
-type kdfAlg_t = prePrfAlg
-type vdAlg_t = protocolVersion * cipherSuite
-
-// Only to be invoked with TLS 1.2 (hardcoded in previous versions)
-// BB.TODO: Documentation ? Confirm that it is used with TLS 1.3 ! CF: no, for TLS 1.3 use tagLen a, e.g. 32 or 64
-// let verifyDataLen_of_ciphersuite (cs:cipherSuite) = 12
-
-// Only to be invoked with TLS 1.2 (hardcoded in previous versions)
-val prfMacAlg_of_ciphersuite_aux: cipherSuite -> Tot (option macAlg)
-let prfMacAlg_of_ciphersuite_aux =
-  let open Hashing.Spec in function
-  | CipherSuite  _ _  (MtE  _ _ )   -> Some (HMac SHA256)
-  | CipherSuite  _ _  (AEAD _ hAlg) -> Some (HMac hAlg)
-  | CipherSuite  _ _  (MACOnly _)   -> Some (HMac SHA256) //MK was (MACOnly hAlg) should it also be be (HMAC hAlg)?
-  | _                               -> None
 
 
-(** Determine if the tuple PV and CS is the correct association with PRF *)
-let pvcs (pv:protocolVersion) (cs:cipherSuite) =
-  match pv, cs with
-  | TLS_1p3, CipherSuite13 _ _ -> true
-  | TLS_1p3, CipherSuite _ _ _ -> false
-  | pv, CipherSuite _ _ _ -> Some? (prfMacAlg_of_ciphersuite_aux cs)
-  | _                 -> false
-
-unfold type require_some (#a:Type) (#b:Type) ($f:(a -> Tot (option b))) =
-  x:a{Some? (f x)} -> Tot b
-
-let prfMacAlg_of_ciphersuite : require_some prfMacAlg_of_ciphersuite_aux =
-  fun x -> Some?.v (prfMacAlg_of_ciphersuite_aux x)
-
-// PRF and verifyData hash algorithms are potentially independent in TLS 1.2,
-// so we use two distinct functions. However, all currently defined ciphersuites
-// use the same hash algorithm, so the current implementation of the two functions
-// is the same.
-
-// Only to be invoked with TLS 1.2 (hardcoded in previous versions
-// BB.TODO: Documentation ? Confirm that it is used with TLS 1.3 !
-let verifyDataHashAlg_of_ciphersuite_aux =
-  let open Hashing.Spec in function
-  | CipherSuite _ _ (MtE  _ _) -> Some SHA256
-  | CipherSuite _ _ (AEAD _ hAlg) -> Some hAlg
-  | CipherSuite _ _ (MACOnly hAlg) -> Some SHA256
-  | CipherSuite13 _ hAlg -> Some hAlg
-  | _ -> None
-
-// BB.TODO: Documentation ?
-let verifyDataHashAlg_of_ciphersuite : require_some verifyDataHashAlg_of_ciphersuite_aux =
-  fun x -> Some?.v (verifyDataHashAlg_of_ciphersuite_aux x)
-
-(** Determine which session hash algorithm is to be used with the protocol version and ciphersuite *)
-val sessionHashAlg: pv:protocolVersion -> cs:cipherSuite{pvcs pv cs} -> Tot hashAlg
-let sessionHashAlg pv cs =
-  match pv with
-  | TLS_1p3 -> let CipherSuite13 _ h = cs in Hash h
-  | SSL_3p0 | TLS_1p0 | TLS_1p1 -> MD5SHA1 // FIXME: DSA uses only SHA1
-  | TLS_1p2 -> Hash (verifyDataHashAlg_of_ciphersuite cs)
-
-// TODO recheck this is the right hash for HKDF
-// SZ: Right. The TLS 1.3 draft says "Where HMAC [RFC2104] uses
-// the Hash algorithm for the handshake"
-
-(** Determine the Authenticated Encryption algorithm associated with a ciphersuite *)
-val get_aeAlg: cs:cipherSuite{ CipherSuite? cs \/ CipherSuite13? cs } -> Tot aeAlg
-let get_aeAlg cs =
-  match cs with
-  | CipherSuite _ _ ae -> ae
-  | CipherSuite13 a h -> AEAD a h
-
-//(** Define the null authenticated encryption algorithm *)
-// BB: Why does this default to MD5 ?
-//let null_aeAlg = MACOnly MD5
-
-(** Determine Encryption type to be used with a chosen PV and AE algorithm *)
-val encAlg_of_aeAlg: (pv:protocolVersion) -> (a:aeAlg { MtE? a }) -> Tot (encAlg * ivMode)
-let encAlg_of_aeAlg  pv ae =
-  match pv,ae with
-  | SSL_3p0, MtE (Block e) m -> (Block e),Stale
-  | TLS_1p0, MtE (Block e) m -> (Block e),Stale
-  | _, MtE e m -> e,Fresh
-
-val macAlg_of_aeAlg: (pv:protocolVersion) -> (a:aeAlg { pv <> TLS_1p3 /\ ~(AEAD? a) }) -> Tot macAlg
-let macAlg_of_aeAlg pv ae =
-  match pv,ae with
-  // 17-02-02 dropping support for weak ciphersuites. To be discussed!
-  //  | SSL_3p0,MACOnly alg -> SSLKHash alg (* dropped pattern on the left to simplify refinements *)
-  //  | SSL_3p0,MtE _ alg   -> SSLKHash alg
-  //  | _      ,MACOnly alg -> SSLKHash alg
-  | _      ,MACOnly alg
-  | _      ,MtE _ alg   -> HMac alg
-
+/// 18-02-22 QD fodder? An auxiliary (largely redundant) enum for
+/// ciphersuites, closer to the RFC and used for configuration in the
+/// TLS APIs.
+/// 
 (** Ciphersuite names definition *)
 type cipherSuiteName =
   | TLS_NULL_WITH_NULL_NULL
@@ -1314,7 +1239,6 @@ let name_of_cipherSuite =
 
   | _ -> Error(AD_illegal_parameter, perror __SOURCE_FILE__ __LINE__ "Invoked on a unknown ciphersuite")
 
-
 #set-options "--max_ifuel 5 --initial_ifuel 5 --max_fuel 1 --initial_fuel 1"
 
 (** Determine the names associated to a list of ciphersuite constructors *)
@@ -1334,10 +1258,131 @@ let rec names_of_cipherSuites css =
       end
     end
 
-// Note:
-// Migrated contentType to Content.fst (this is internal to TLS)
 
 
+
+
+// Some of these could be hidden in Handshake.Secret
+
+(** Definition for the PRF label type *)
+type prflabel = bytes
+
+(** Key schedule labels *)
+let extract_label          = utf8_encode "master secret"
+let extended_extract_label = utf8_encode "extended master secret"
+let kdf_label              = utf8_encode "key expansion"
+
+(** PRF definitions based on the protocol version *)
+type prePrfAlg =
+  | PRF_SSL3_nested         // MD5(SHA1(...)) for extraction and keygen
+  | PRF_SSL3_concat         // MD5 @| SHA1    for VerifyData tags
+  | PRF_TLS_1p01 of prflabel                       // MD5 xor SHA1
+  | PRF_TLS_1p2 : prflabel -> macAlg -> prePrfAlg  // typically SHA256 but may depend on CS
+  | PRF_TLS_1p3 // TBC
+
+(** PRF associations *)
+//BB.TODO: Documentation ?
+type kefAlg_t = prePrfAlg
+type kdfAlg_t = prePrfAlg
+type vdAlg_t = protocolVersion * cipherSuite
+
+// Only to be invoked with TLS 1.2 (hardcoded in previous versions)
+// BB.TODO: Documentation ? Confirm that it is used with TLS 1.3 ! CF: no, for TLS 1.3 use tagLen a, e.g. 32 or 64
+// let verifyDataLen_of_ciphersuite (cs:cipherSuite) = 12
+
+// Only to be invoked with TLS 1.2 (hardcoded in previous versions)
+val prfMacAlg_of_ciphersuite_aux: cipherSuite -> Tot (option macAlg)
+let prfMacAlg_of_ciphersuite_aux =
+  let open Hashing.Spec in function
+  | CipherSuite  _ _  (MtE  _ _ )   -> Some (HMac SHA256)
+  | CipherSuite  _ _  (AEAD _ hAlg) -> Some (HMac hAlg)
+  | CipherSuite  _ _  (MACOnly _)   -> Some (HMac SHA256) //MK was (MACOnly hAlg) should it also be be (HMAC hAlg)?
+  | _                               -> None
+
+(** Determine if the tuple PV and CS is the correct association with PRF *)
+let pvcs (pv:protocolVersion) (cs:cipherSuite) =
+  match pv, cs with
+  | TLS_1p3, CipherSuite13 _ _ -> true
+  | TLS_1p3, CipherSuite _ _ _ -> false
+  | pv, CipherSuite _ _ _ -> Some? (prfMacAlg_of_ciphersuite_aux cs)
+  | _                 -> false
+
+unfold type require_some (#a:Type) (#b:Type) ($f:(a -> Tot (option b))) =
+  x:a{Some? (f x)} -> Tot b
+
+let prfMacAlg_of_ciphersuite : require_some prfMacAlg_of_ciphersuite_aux =
+  fun x -> Some?.v (prfMacAlg_of_ciphersuite_aux x)
+
+// PRF and verifyData hash algorithms are potentially independent in TLS 1.2,
+// so we use two distinct functions. However, all currently defined ciphersuites
+// use the same hash algorithm, so the current implementation of the two functions
+// is the same.
+
+// Only to be invoked with TLS 1.2 (hardcoded in previous versions
+// BB.TODO: Documentation ? Confirm that it is used with TLS 1.3 !
+private 
+let verifyDataHashAlg_of_ciphersuite_aux =
+  let open Hashing.Spec in function
+  | CipherSuite _ _ (MtE  _ _) -> Some SHA256
+  | CipherSuite _ _ (AEAD _ hAlg) -> Some hAlg
+  | CipherSuite _ _ (MACOnly hAlg) -> Some SHA256
+  | CipherSuite13 _ hAlg -> Some hAlg
+  | _ -> None
+
+// BB.TODO: Documentation ?
+let verifyDataHashAlg_of_ciphersuite : require_some verifyDataHashAlg_of_ciphersuite_aux =
+  fun x -> Some?.v (verifyDataHashAlg_of_ciphersuite_aux x)
+
+(** Determine which session hash algorithm is to be used with the protocol version and ciphersuite *)
+val sessionHashAlg: pv:protocolVersion -> cs:cipherSuite{pvcs pv cs} -> Tot hashAlg
+let sessionHashAlg pv cs =
+  match pv with
+  | TLS_1p3 -> let CipherSuite13 _ h = cs in Hash h
+  | SSL_3p0 | TLS_1p0 | TLS_1p1 -> MD5SHA1 // FIXME: DSA uses only SHA1
+  | TLS_1p2 -> Hash (verifyDataHashAlg_of_ciphersuite cs)
+
+// TODO recheck this is the right hash for HKDF
+// SZ: Right. The TLS 1.3 draft says "Where HMAC [RFC2104] uses
+// the Hash algorithm for the handshake"
+
+(** Determine the Authenticated Encryption algorithm associated with a ciphersuite *)
+val get_aeAlg: cs:cipherSuite{ CipherSuite? cs \/ CipherSuite13? cs } -> Tot aeAlg
+let get_aeAlg cs =
+  match cs with
+  | CipherSuite _ _ ae -> ae
+  | CipherSuite13 a h -> AEAD a h
+
+//(** Define the null authenticated encryption algorithm *)
+// BB: Why does this default to MD5 ?
+//let null_aeAlg = MACOnly MD5
+
+(** Determine Encryption type to be used with a chosen PV and AE algorithm *)
+val encAlg_of_aeAlg: (pv:protocolVersion) -> (a:aeAlg { MtE? a }) -> Tot (encAlg * ivMode)
+let encAlg_of_aeAlg  pv ae =
+  match pv,ae with
+  | SSL_3p0, MtE (Block e) m -> (Block e),Stale
+  | TLS_1p0, MtE (Block e) m -> (Block e),Stale
+  | _, MtE e m -> e,Fresh
+
+val macAlg_of_aeAlg: (pv:protocolVersion) -> (a:aeAlg { pv <> TLS_1p3 /\ ~(AEAD? a) }) -> Tot macAlg
+let macAlg_of_aeAlg pv ae =
+  match pv,ae with
+  // 17-02-02 dropping support for weak ciphersuites. To be discussed!
+  //  | SSL_3p0,MACOnly alg -> SSLKHash alg (* dropped pattern on the left to simplify refinements *)
+  //  | SSL_3p0,MtE _ alg   -> SSLKHash alg
+  //  | _      ,MACOnly alg -> SSLKHash alg
+  | _      ,MACOnly alg
+  | _      ,MtE _ alg   -> HMac alg
+
+
+
+
+
+
+
+
+/// 18-02-22 QD fodder
+/// 
 (** Certificate type definition *)
 type certType =
   | RSA_sign
@@ -1364,7 +1409,6 @@ let parseCertType b =
   | 4z -> Correct DSA_fixed_dh
   | _ -> Error(AD_decode_error, perror __SOURCE_FILE__ __LINE__ "")
 
-
 (** Lemmas associated to serializing/parsing of certificate types *)
 val inverse_certType: x:_ -> Lemma
   (requires True)
@@ -1377,7 +1421,6 @@ val pinverse_certType: x:_ -> Lemma
   (ensures (lemma_pinverse_f_g Bytes.equal certTypeBytes parseCertType x))
   [SMTPat (certTypeBytes (Correct?._0 (parseCertType x)))]
 let pinverse_certType x = ()
-
 
 #set-options "--max_fuel 1 --initial_fuel 1"
 
@@ -1403,9 +1446,7 @@ let rec parseCertificateTypeList data =
       let rem = parseCertificateTypeList data in
       ct :: rem
 
-
 #set-options "--max_ifuel 4 --initial_ifuel 1 --max_fuel 4 --initial_fuel 1"
-
 
 (** Determine the certificate signature algorithms allowed according to the ciphersuite *)
 val defaultCertTypes: bool -> cipherSuite -> ML (l:list certType{List.Tot.length l <= 1})
@@ -1423,9 +1464,7 @@ let defaultCertTypes sign cs =
       | DSA -> [DSA_fixed_dh]
       | _ -> unexpected "[defaultCertTypes] invoked on an invalid ciphersuite"
 
-
 #set-options "--max_ifuel 2 --initial_ifuel 2 --max_fuel 1 --initial_fuel 1"
-
 
 (** Type definition of the Distinguished Name of a certificate *)
 type dn = s:string{length(utf8_encode s) < 256}
@@ -1462,9 +1501,10 @@ let rec parseDistinguishedNameList data res =
     else Error(AD_decode_error, perror __SOURCE_FILE__ __LINE__ "")
         end
 
-(** Determine if a ciphersuite list contains the SCSV ciphersuite *)
-let contains_TLS_EMPTY_RENEGOTIATION_INFO_SCSV (css: list cipherSuite) =
-  List.Tot.mem (SCSV (TLS_EMPTY_RENEGOTIATION_INFO_SCSV)) css
+
+
+
+
 
 // TODO: move all the definitions below to a separate file / figure out whether
 // they belong here ?
@@ -1472,124 +1512,13 @@ let contains_TLS_EMPTY_RENEGOTIATION_INFO_SCSV (css: list cipherSuite) =
 // TODO: all occurrences of [pinverse] from there on have been replaced by calls
 // to [pinverse_t]; we should write corresponding inversion lemmas.
 
-(** Definition of the configuration identifier *)
-type configurationId = b:bytes{0 < length b /\ length b < 65536}
-
-(** Serializing function for the configuration identifier *)
-val configurationIdBytes: configurationId -> Tot (b:bytes{2 < length b /\ length b < 65538})
-let configurationIdBytes cid =
-  lemma_repr_bytes_values (length cid);
-  vlbytes 2 cid
-
-(** Parsing function for the configuration identifier *)
-val parseConfigurationId: pinverse_t configurationIdBytes
-let parseConfigurationId b =
-  match vlparse 2 b with
-  | Error z -> Error z
-  | Correct b -> Correct b
-
-(** Lemmas for configurationId serializing/parsing inversion *)
-val inverse_configurationId: x:_ -> Lemma
-  (requires True)
-  (ensures lemma_inverse_g_f configurationIdBytes parseConfigurationId x)
-  [SMTPat (parseConfigurationId (configurationIdBytes x))]
-let inverse_configurationId x =
-  lemma_repr_bytes_values (length x)
-
-val pinverse_configurationId: x:_ -> Lemma
-  (requires True)
-  (ensures (lemma_pinverse_f_g Bytes.equal configurationIdBytes parseConfigurationId x))
-  [SMTPat (configurationIdBytes (Correct?._0 (parseConfigurationId x)))]
-let pinverse_configurationId x = ()
-
-// TODO: replace with more precise types when available
-(** Configuration Extension definition *)
-noeq type configurationExtension =
-  | UnknownConfigurationExtension:
-      typ:lbytes 2 -> payload: bytes { repr_bytes (length payload) <= 2 } -> configurationExtension
-
-// TODO: Should we strengthen the result type to b:bytes{length b >= 4}?
-(** Serialization of the configuration extension values *)
-val configurationExtensionBytes: ce:configurationExtension -> Tot bytes
-let configurationExtensionBytes ce =
-  match ce with
-  | UnknownConfigurationExtension typ payload -> typ @| vlbytes 2 payload
-
-(** Parsing of the configuration extension values *)
-val parseConfigurationExtension: pinverse_t configurationExtensionBytes
-let parseConfigurationExtension b =
-  if length b >= 4 then
-    let (typ,payload) = split b 2ul in
-    match vlparse 2 payload with
-    | Correct payload -> Correct (UnknownConfigurationExtension typ payload)
-    | Error z -> Error z
-  else Error (AD_decode_error, perror __SOURCE_FILE__ __LINE__ "Too few bytes to parse a configuration extension")
 
 
-(** Lemmas for Configuration Extension parsing/serializing inversions *)
-val inverse_configurationExtension: x:_ -> Lemma
-  (requires True)
-  (ensures lemma_inverse_g_f configurationExtensionBytes parseConfigurationExtension x)
-  [SMTPat (parseConfigurationExtension (configurationExtensionBytes x))]
-let inverse_configurationExtension x =
-  match x with
-  | UnknownConfigurationExtension typ payload ->
-  let b = typ @| vlbytes 2 payload in
-  let b0,b1 = split b 2ul in
-  let vl,b = split b1 2ul in
-  vlparse_vlbytes 2 b;
-  assert (Bytes.equal vl (bytes_of_int 2 (length b)));
-  assert (Bytes.equal b0 typ);
-  assert (Bytes.equal b payload)
-
-val pinverse_configurationExtension: x:_ -> Lemma
-  (requires True)
-  (ensures (lemma_pinverse_f_g Bytes.equal configurationExtensionBytes parseConfigurationExtension x))
-  [SMTPat (configurationExtensionBytes (Correct?._0 (parseConfigurationExtension x)))]
-let pinverse_configurationExtension x = ()
 
 
-// TODO: Choice, truncate when maximum length is exceeded
-(** Serialization of the configuration extension list of values *)
-let rec configurationExtensionsBytes_aux (b:bytes{length b < 65536}) (ces:list configurationExtension): Tot (b:bytes{length b < 65536}) (decreases ces) =
-  match ces with
-  | [] -> b
-  | ce::ces ->
-    if length (b @| configurationExtensionBytes ce) < 65536 then
-      configurationExtensionsBytes_aux (b @| configurationExtensionBytes ce) ces
-    else b
 
-val configurationExtensionsBytes: list configurationExtension -> Tot bytes
-let configurationExtensionsBytes ce =
-  let b = configurationExtensionsBytes_aux empty_bytes ce in
-  lemma_repr_bytes_values (length b);
-  vlbytes 2 b
-
-(** Parsing of the configuration extension list of values *)
-let rec parseConfigurationExtensions_aux (b:bytes) (exts:list configurationExtension)
-  : Tot (result (list configurationExtension)) (decreases (length b))
-  = if length b > 0 then
-      if length b >= 4 then
-        let typ, len_data = split b 2ul in
-        let len, data = split len_data 2ul in
-        let len = int_of_bytes len in
-        if length b >= 4 + len then
-          let ext, bytes = split_ b len in
-          match parseConfigurationExtension ext with
-          | Correct(ext') -> parseConfigurationExtensions_aux bytes (ext'::exts)
-          | Error(z) -> Error(z)
-        else Error(AD_decode_error, perror __SOURCE_FILE__ __LINE__ "Failed to parse configuration extension length")
-      else Error(AD_decode_error, perror __SOURCE_FILE__ __LINE__ "Configuration extension length should be at least 4")
-    else Correct(exts)
-
-val parseConfigurationExtensions: pinverse_t configurationExtensionsBytes
-let parseConfigurationExtensions b =
-  if length b >= 2 then
-  match vlparse 2 b with
-  | Correct (b) ->  parseConfigurationExtensions_aux b []
-  | Error(z) -> Error(AD_decode_error, perror __SOURCE_FILE__ __LINE__ "Failed to parse configuration extension")
-  else Error(AD_decode_error, perror __SOURCE_FILE__ __LINE__ "Failed to parse configuration extension")
-
+/// 18-02-22 QD fodder
+/// 
 let signatureSchemeList =
   algs:list signatureScheme{0 < List.Tot.length algs /\ op_Multiply 2 (List.Tot.length algs) < 65536}
 
@@ -1665,7 +1594,6 @@ val parseSignatureSchemeList: pinverse_t signatureSchemeListBytes
       else Error (AD_decode_error, perror __SOURCE_FILE__ __LINE__ "Too few bytes to parse sig hash algs")
     else Correct algs
 
-
 let parseSignatureSchemeList b =
   match vlparse 2 b with
   | Correct b ->
@@ -1677,32 +1605,9 @@ let parseSignatureSchemeList b =
   | Error z -> Error(AD_decode_error, perror __SOURCE_FILE__ __LINE__ "Failed to parse sig hash algs")
 
 
-(*
-// We use a non-tail recursive version in Extensions.fst
-let parseSupportedVersions b =
-  let rec aux: b:bytes -> pvs:list protocolVersion{length b + op_Multiply 2 (List.Tot.length pvs) < 65536} -> Tot (result (l:list protocolVersion{List.Tot.length l < 65536/2}))
-  (decreases (length b)) = fun b pvs ->
-    if length b > 0 then
-      if length b >= 2 then
-      let pv, bytes = split b 2 in
-      match parseProtocolVersion pv with
-      | Correct pv -> aux bytes (pv :: pvs)
-      | Error z    -> Error z
-      else Error (AD_decode_error, perror __SOURCE_FILE__ __LINE__ "Too few bytes to parse protocol version")
-    else Correct pvs
-  in
-  match vlparse 2 b with
-  | Correct b ->
-    begin
-    match aux b [] with
-    | Correct [] ->
-      Error(AD_decode_error, perror __SOURCE_FILE__ __LINE__ "Empty list of protocol versions")
-    | Correct pvs -> Correct pvs
-    | Error z -> Error z
-    end
-  | Error z ->
-    Error(AD_decode_error, perror __SOURCE_FILE__ __LINE__ "Failed to parse protocol versions")
-*)
+
+
+
 
 
 // Moved here because it's used in both Extensions and TLSInfo and Extensions
@@ -1742,11 +1647,23 @@ Certificate Request?
 type ServerCertificateRequest // something that determines this Handshake message
 
 request_client_certificate: single_assign ServerCertificateRequest // uses this one, or asks the server; by default Some None.
-
 *)
+
+
+
+
+
+/// 18-02-22 QD fodder; their formatting is in Extensions.
+/// 
 type alpn_entry = b:bytes{0 < length b /\ length b < 256}
 type alpn = l:list alpn_entry{List.Tot.length l < 256}
 
+
+
+
+
+/// 18-02-22 QD fodder; their formatting is in Extensions.
+/// 
 type quicParameter =
   | Quic_initial_max_stream_data of UInt32.t
   | Quic_initial_max_data of UInt32.t
@@ -1817,6 +1734,12 @@ let string_of_quicParameters = function
     string_of_quicParameters_aux_fold "" string_of_quicParameter "\n" p
   | None -> "(none)"
 
+
+
+
+
+
+
 type pskInfo = {
   ticket_nonce: option bytes;
   time_created: int;
@@ -1845,8 +1768,7 @@ noeq type ticket_cb = {
 type cert_repr = b:bytes {length b < 16777216}
 type cert_type = FFICallbacks.callbacks
 
-noeq
-abstract
+noeq abstract
 type cert_cb = {
   app_context : FStar.Dyn.dyn;
   (* Each callback takes an application context (app_context)
@@ -1886,24 +1808,24 @@ type cert_cb = {
 }
 
 let mk_cert_cb
-      app_ctx
-      cert_select_ptr
-      cert_select_cb
-      cert_format_ptr
-      cert_format_cb
-      cert_sign_ptr
-      cert_sign_cb
-      cert_verify_ptr
-      cert_verify_cb = {
-    app_context  = app_ctx;
-    cert_select_ptr = cert_select_ptr;
-    cert_select_cb = cert_select_cb;
-    cert_format_ptr = cert_format_ptr;
-    cert_format_cb = cert_format_cb;
-    cert_sign_ptr = cert_sign_ptr;
-    cert_sign_cb = cert_sign_cb;
-    cert_verify_ptr = cert_verify_ptr;
-    cert_verify_cb = cert_verify_cb
+    app_ctx
+    cert_select_ptr
+    cert_select_cb
+    cert_format_ptr
+    cert_format_cb
+    cert_sign_ptr
+    cert_sign_cb
+    cert_verify_ptr
+    cert_verify_cb = {
+  app_context  = app_ctx;
+  cert_select_ptr = cert_select_ptr;
+  cert_select_cb = cert_select_cb;
+  cert_format_ptr = cert_format_ptr;
+  cert_format_cb = cert_format_cb;
+  cert_sign_ptr = cert_sign_ptr;
+  cert_sign_cb = cert_sign_cb;
+  cert_verify_ptr = cert_verify_ptr;
+  cert_verify_cb = cert_verify_cb
 }
 
 noeq type config : Type0 = {
@@ -1982,19 +1904,4 @@ type cVerifyData = b:bytes{length b <= 64} (* ClientFinished payload *)
 type sVerifyData = b:bytes{length b <= 64} (* ServerFinished payload *)
 
 
-// -------------------------------------------------------------------
-// We support these extensions, with session scopes
-// (defined here because TLSExtension is internal)
 
-type ri_status =
-| RI_Unsupported
-| RI_Valid
-| RI_Invalid
-
-type serverName =
-| SNI_DNS of b:bytes{repr_bytes (length b) <= 2}
-| SNI_UNKNOWN of (n:nat{repr_bytes n <= 1}) * (b:bytes{repr_bytes (length b) <= 2})
-
-type point_format =
-  | ECP_UNCOMPRESSED
-  | ECP_UNKNOWN of (n:nat{repr_bytes n <= 1})
